Dex001/README.md
@@ -6,7 +6,30 @@
 To verify/record hints, run `zebra  --z3rlimit 7000000 -e Dex001.fst`.  
 This command may take a long time to run the first time.
 Subsequent runs will be significantly faster.
-With an AMD Threadripper 1950x @4.0GHz, recording hints takes ~67s. Subsequent runs take ~11s.
+With an AMD Threadripper 1950x @4.0GHz, recording hints can take up to 2 minutes. Subsequent runs take ~11s.
+
+## How it works
+
+ZenDex is a true decentralised exchange, with no operator or fees.
+
+ZenDex stores orders as utxos that it locks to itself.
+In this manner, we avoid having a shared state, allowing great parallelism.
+
+When an order is made, the order parameters are hashed together.
+ZenDex mints and single token with that hash as it's sub-identifier (the '*order asset*'),
+and locks that to itself.
+
+When an order is taken or cancelled, that token is destroyed.
+In the case of a partial fill,
+ZenDex will create a new order with reduced quantities of the underlying and order total.
+The previous order is still destroyed.
+
+When cancelling or taking an order,
+one must supply all of the order parameters directly to ZenDex in the messageBody,
+because ZenDex does not store this information, and only possesses a hash of the order.
+
+Order books can be constructed by folding over the blockchain,
+and looking for transactions involving ZenDex.
 
 ## Usage
 
@@ -37,7 +60,7 @@ For example, to make an order selling 50ZP for 1234 of some asset α which has a
 The messageBody would include the field-value pairs
 
 | Field Name | Type | Value | Notes |
-|:----------:|:----:| ----------- | ----- |
+|:----------:|:----:|:-----------:| ----------------------------------------------------- |
 | `"UnderlyingAssetVersion"` | `UInt32` | 0 | The ZP asset has version 0 |
 | `"UnderlyingContractHash"` | `Hash`   | `0000000000000000000000000000000000000000000000000000000000000000` | The ZP asset has the zero hash as it's contract hash |
 | `"UnderlyingContractHash"` | `Hash`   | `0000000000000000000000000000000000000000000000000000000000000000` | The ZP asset has the zero hash as it's asset sub-identifier |
@@ -59,14 +82,51 @@ The messageBody must consist of a dictionary which includes the following fields
 | `"UnderlyingAssetVersion"` | `UInt32` | The version number of the underlying asset of your order |
 | `"UnderlyingContractHash"` | `Hash`   | The contract hash for the underlying asset of your order |
 | `"UnderlyingSubIdentifier"`| `Hash`   | The asset sub-identifier for the underlying asset of your order |
-| `"UnderlyingAmount"` | `Hash` | The amount of the underlying in the order |
+| `"UnderlyingAmount"` | `UInt64` | The amount of the underlying in the order |
 | `"PairAssetVersion"` | `UInt32` | The version number of the pair asset of your order |
 | `"PairContractHash"` | `Hash` | The contract hash for the pair asset of your order |
 | `"PairSubIdentifier"` | `Hash` | The asset sub-identifier for the pair asset of your order |
-| `"OrderTotal"` | `UInt64` | The total amount of the pair ordered |
+| `"OrderTotal"` | `UInt64` | The total amount of the pair requested in the order |
 
-the transaction must place the order asset in ZenDex's contract wallet.
+The transaction must place the order asset in ZenDex's contract wallet,
+as well as a sufficient quantity of the underlying.
 
 ### Taking an order
 
 Use the command `"Take"`.
+
+The messageBody must consist of a dictionary which includes the following fields:
+
+| Field Name | Type | Description |
+|:----------:|:----:| ----------- |
+| `"UnderlyingAssetVersion"` | `UInt32` | The version number of the underlying asset of the order being taken |
+| `"UnderlyingContractHash"` | `Hash`   | The contract hash for the underlying asset of the order being taken |
+| `"UnderlyingSubIdentifier"`| `Hash`   | The asset sub-identifier for the underlying asset of the order being taken |
+| `"UnderlyingAmount"` | `UInt64` | The amount of the underlying in the order |
+| `"PairAssetVersion"` | `UInt32` | The version number of the pair asset of the order being taken |
+| `"PairContractHash"` | `Hash` | The contract hash for the pair asset of the order being taken |
+| `"PairSubIdentifier"` | `Hash` | The asset sub-identifier for the pair asset of the order being taken |
+| `"OrderTotal"` | `UInt64` | The total amount of the pair requested in the order |
+| `"MakerPK"` | `PublicKey` | The public key of the maker of the order being taken |
+| `"RequestedPayout"` | `UInt64` | The amount of the underlying to pay out |
+
+The transaction must place the order asset being taken and a sufficient amount of the underlying in ZenDex's contract wallet,
+and must lock an amount α of the order's pair asset to the contract, where
+<img src="https://latex.codecogs.com/svg.latex?\texttt{RequestedPayout}&space;=&space;\left&space;\lfloor{\texttt{UnderlyingAmount}&space;\times&space;\frac{\alpha}{\texttt{OrderTotal}}}&space;\right&space;\rfloor" title="\texttt{RequestedPayout} = \left \lfloor{\texttt{UnderlyingAmount} \times \frac{\alpha}{\texttt{OrderTotal}}} \right \rfloor" />.
+
+## Notes
+
+Orders are expressed in terms of underlying amount and pair amount to allow for rational price ratios - eg. a trade of 5α for 7β, or 13β for 11γ.
+This is not easily expressed as a 'price per' with only integer arithmetic.
+The payout for a partial fill should, assuming arbitrarily divisible assets, be calculated as
+<img src="https://latex.codecogs.com/svg.latex?\texttt{Payout}&space;=&space;\texttt{UnderlyingAmount}&space;\times&space;\frac{\texttt{PaymentAmount}}{\texttt{OrderTotal}}" title="\texttt{Payout} = \texttt{UnderlyingAmount} \times \frac{\texttt{PaymentAmount}}{\texttt{OrderTotal}}" />.
+However, since we do not have arbitrarily divisible assets, we denote orders in the smallest unit of each asset and compute the floor, so that
+<img src="https://latex.codecogs.com/svg.latex?\texttt{Payout}&space;=&space;\left&space;\lfloor{\texttt{UnderlyingAmount}&space;\times&space;\frac{\texttt{PaymentAmount}}{\texttt{OrderTotal}}}&space;\right&space;\rfloor" title="\texttt{Payout} = \left \lfloor{\texttt{UnderlyingAmount} \times \frac{\texttt{PaymentAmount}}{\texttt{OrderTotal}}} \right \rfloor" />.
+
+The underlying amount, order total, and payment amount are all 64 bit unsigned integers.
+Version 0 ZF* contracts lack integer representations larger than this, and so we are tasked with implementing double-word arithmetic in order to calculate the payoff.
+In order to avoid the complexity and potential for error in implementing double-word division,
+we instead ask the user to provide the payoff, and validate that it is correct.
+Validating that a user's `RequestedPayout` is correct is simpler than computing the payout,
+and requires only double-word multiplication and comparison,
+both relatively simple compared to double-word division.
